more cleanup.
- removing dead files
- adding quantifiers
- adding proofs for multimem

src/MultiMem.v
@@ -1,3 +1,8 @@
+Require Import Heaps.
+
+Set Implicit Arguments.
+Set Strict Implicit.
+
 Section parametric.
   Variable T : Type.
 
@@ -13,14 +18,14 @@ Section multi_mem.
   Variables mem addr val : Type.
 
   Section read.
-    Variable read : mem -> addr -> option val.
+    Variable read : addr -> mem -> option val.
     Variable m : mem.
   
     Fixpoint multi_read_addrs (n : nat) : vector addr n -> (vector val n -> T) -> option T :=
       match n as n return vector addr n -> (vector val n -> T) -> option T with
         | 0 => fun _ k => Some (k tt)
         | S n => fun a k =>
-          match read m (fst a) with
+          match read (fst a) m with
             | None => None
             | Some v => multi_read_addrs n (snd a) (fun vs => k (v,vs))
           end
@@ -46,7 +51,7 @@ Section multi_mem.
   Variable implode : vector val N -> T.
   Variable explode : T -> vector val N.
 
-  Definition multi_read (read : mem -> addr -> option val) (a : addr) (m : mem) : option T :=
+  Definition multi_read (read : addr -> mem -> option val) (a : addr) (m : mem) : option T :=
     multi_read_addrs read m N (footprint a) implode.
 
   Definition multi_write (write : addr -> val -> mem -> option mem) (a : addr) (v : T) : mem -> option mem :=
@@ -54,3 +59,64 @@ Section multi_mem.
   
 End multi_mem.
 
+Module MultiSepMemFacts (SM : SeparationMemory).
+  
+  Lemma split_smem_read_multi' : forall T (N : nat) k a b c addrs v,
+    SM.split a b c ->
+      @multi_read_addrs T SM.smem SM.M.addr SM.M.value SM.smem_get b N addrs k = Some v ->
+      @multi_read_addrs T SM.smem SM.M.addr SM.M.value SM.smem_get a N addrs k = Some v.
+  Proof.
+    induction N; simpl; intros; auto.
+    revert H0.
+    match goal with
+      | [ |- match ?X with _ => _ end = _ -> _ ] =>
+        case_eq X; intros; try congruence
+    end.
+    eapply SM.split_smem_get in H0; eauto.
+    rewrite H0. eauto.
+  Qed.
+
+  Lemma split_smem_write_multi' : forall (N : nat) addrs vals a b c b',
+    SM.split a b c ->
+      @multi_write_addrs SM.smem SM.M.addr SM.M.value SM.smem_set N addrs vals b = Some b' ->
+      exists a', SM.split a' b' c /\
+        @multi_write_addrs SM.smem SM.M.addr SM.M.value SM.smem_set N addrs vals a = Some a'.
+  Proof.
+    induction N; simpl; intros; auto.
+    { inversion H0; subst; eauto. }
+    { revert H0.
+      match goal with
+        | [ |- match ?X with _ => _ end = _ -> _ ] =>
+          case_eq X; intros; try congruence
+      end.
+      eapply SM.split_smem_set in H0; eauto.
+      destruct H0. intuition. rewrite H3.
+      eauto. }
+  Qed.
+
+  Section exposed.
+    Variable T : Type.
+    Variable N : nat.
+    Variable footprint : SM.M.addr -> vector SM.M.addr N.
+    Variable implode : vector SM.M.value N -> T.
+    Variable explode : T -> vector SM.M.value N.
+
+    Theorem split_multi_read : forall a b c p v,
+      SM.split a b c ->
+        @multi_read T SM.smem SM.M.addr SM.M.value N footprint implode SM.smem_get p b = Some v ->
+        @multi_read T SM.smem SM.M.addr SM.M.value N footprint implode SM.smem_get p a = Some v.
+    Proof.
+      intros. eapply split_smem_read_multi'; eauto.
+    Qed.
+
+    Theorem split_multi_write : forall p v a b c b',
+    SM.split a b c ->
+      @multi_write T SM.smem SM.M.addr SM.M.value N footprint explode SM.smem_set p v b = Some b' ->
+      exists a', SM.split a' b' c /\
+        @multi_write T SM.smem SM.M.addr SM.M.value N footprint explode SM.smem_set p v a = Some a'.
+    Proof.
+      intros. eapply split_smem_write_multi'; eauto.
+    Qed.
+  End exposed.
+
+End MultiSepMemFacts.
