src/Quantifier.v
@@ -1,0 +1,190 @@
+Require Import List.
+Require Import Expr.
+
+Set Implicit Arguments.
+Set Strict Implicit.
+
+Section over_types.
+  Variable types : list type.
+
+  Inductive Quant : Type := 
+  | QAll  : variables -> Quant -> Quant
+  | QEx   : variables -> Quant -> Quant
+  | QBase : Quant.
+
+  (** NOTE: For efficiency, the outer-most quantifier should be
+   ** the deepest quantifier
+   **)
+  (** NOTE: 
+   ** For forward reasoning we need to invert the quantifiers.
+   ** i.e. All quantifiers should become uvar and 
+   **      Ex quantifiers should become var
+   **)
+  Fixpoint quantD (ex_env all_env : env types) (qs : Quant) (k : env types -> env types -> Prop) : Prop :=
+    match qs with
+      | QBase => k ex_env all_env
+      | QAll vs qs => quantD ex_env all_env qs (fun ex_env all_env => forallEach vs (fun all_ext => k ex_env (all_env ++ all_ext)))
+      | QEx vs qs => quantD ex_env all_env qs (fun ex_env all_env => existsEach vs (fun ex_ext => k (ex_env ++ ex_ext) all_env))
+    end.
+
+  Fixpoint appendQ (q1 q2 : Quant) : Quant :=
+    match q1 with 
+      | QBase => q2
+      | QAll vs q1 => QAll vs (appendQ q1 q2)
+      | QEx vs q1 => QEx vs (appendQ q1 q2)
+    end.
+
+  Theorem quantD_app : forall qs' qs meta_env vars_env k, 
+    quantD meta_env vars_env (appendQ qs qs') k <->
+    quantD meta_env vars_env qs' (fun meta_env vars_env => quantD meta_env vars_env qs k).
+  Proof.
+    clear; induction qs; simpl; intros; try rewrite IHqs; try reflexivity.
+  Qed.
+
+  Fixpoint gatherEx (qs : Quant) : variables :=
+    match qs with
+      | QBase => nil
+      | QAll _ qs => gatherEx qs
+      | QEx vs qs => gatherEx qs ++ vs
+    end.
+
+  Fixpoint gatherAll (qs : Quant) : variables :=
+    match qs with
+      | QBase => nil
+      | QAll vs qs => gatherAll qs ++ vs
+      | QEx _ qs => gatherAll qs
+    end.
+
+  Theorem quantD_impl : forall qs meta_env vars_env (k k' : _ -> _ -> Prop),
+    quantD meta_env vars_env qs k ->
+    (forall a b,
+      typeof_env a = gatherEx qs -> 
+      typeof_env b = gatherAll qs -> 
+      k (meta_env ++ a) (vars_env ++ b) ->
+      k' (meta_env ++ a) (vars_env ++ b)) ->
+    quantD meta_env vars_env qs k'.
+  Proof.
+    clear. induction qs; simpl; intros; try (eapply IHqs; [ eauto | ]); simpl in *; intros; instantiate; simpl in *;
+    repeat match goal with 
+             | [ |- existsEach _ _ ] => eapply existsEach_sem
+             | [ |- forallEach _ _ ] => eapply forallEach_sem; intros
+             | [ H : existsEach _ _ |- _ ] =>
+               eapply existsEach_sem in H; destruct H
+             | [ H : forallEach _ _ |- _ ] =>
+               eapply forallEach_sem in H; [ | solve [ eauto ] ]
+             | [ H : _ /\ _ |- _ ] => destruct H
+             | [ |- exists x, _ /\ _ ] =>
+               eexists; split; [ solve [ eauto ] | ]                   
+             | [ |- _ ] => rewrite app_ass in *
+           end.
+    { eapply H0; eauto. subst. rewrite <- H2. unfold typeof_env. rewrite map_app. auto. }
+    { eapply H0; eauto. subst. rewrite <- H1. unfold typeof_env. rewrite map_app. auto. }
+    { specialize (H0 nil nil). repeat rewrite app_nil_r in *. auto. }
+  Qed.
+
+  Require Import Tactics.
+
+  Theorem gatherEx_appendQ : forall q1 q2, 
+    gatherEx (appendQ q1 q2) = gatherEx q2 ++ gatherEx q1.
+  Proof.
+    induction q1; simpl; intros; think; repeat (rewrite app_nil_r || rewrite app_ass); auto.
+  Qed.
+
+  Theorem gatherAll_appendQ : forall q1 q2, 
+    gatherAll (appendQ q1 q2) = gatherAll q2 ++ gatherAll q1.
+  Proof.
+    induction q1; simpl; intros; think; repeat (rewrite app_nil_r || rewrite app_ass); auto.
+  Qed.
+
+  Definition qex (ls : list tvar) (q : Quant) : Quant :=
+    match ls with
+      | nil => q
+      | _ => QEx ls q
+    end.
+
+  Definition qall (ls : list tvar) (q : Quant) : Quant :=
+    match ls with
+      | nil => q
+      | _ => QAll ls q
+    end.
+
+  Lemma quantD_qex_QEx : forall U G a b P,
+    quantD U G (QEx a b) P <-> quantD U G (qex a b) P.
+  Proof. clear.
+    destruct a; simpl in *; split; intros; auto.
+    { eapply quantD_impl; eauto; intros. simpl in *. rewrite app_nil_r in *. auto. }
+    { eapply quantD_impl; eauto; intros. simpl in *. rewrite app_nil_r in *. auto. }
+  Qed.
+
+  Lemma quantD_qall_QAll : forall U G a b P,
+    quantD U G (QAll a b) P <-> quantD U G (qall a b) P.
+  Proof. clear.
+    destruct a; simpl in *; split; intros; auto.
+    { eapply quantD_impl; eauto; intros. simpl in *. rewrite app_nil_r in *. auto. }
+    { eapply quantD_impl; eauto; intros. simpl in *. rewrite app_nil_r in *. auto. }
+  Qed.
+
+  Lemma appendQ_assoc : forall a b c,
+    appendQ (appendQ a b) c = appendQ a (appendQ b c).
+  Proof.
+    clear. induction a; simpl; intros; try f_equal; eauto.
+  Qed.
+
+  Lemma appendQ_QAll : forall a b v,
+    appendQ a (QAll v b) = appendQ (appendQ a (QAll v QBase)) b.
+  Proof. clear.
+    induction a; simpl; intros; try rewrite IHa; eauto.
+  Qed.
+  Lemma appendQ_QEx : forall a b v,
+    appendQ a (QEx v b) = appendQ (appendQ a (QEx v QBase)) b.
+  Proof. clear.
+    induction a; simpl; intros; try rewrite IHa; eauto.
+  Qed.
+
+  Lemma QAll_inj_False : forall a b,
+    QAll a b = b -> False.
+  Proof. clear.
+    induction b; simpl; intros; try congruence; auto.
+  Qed.
+
+  Lemma QEx_inj_False : forall a b,
+    QEx a b = b -> False.
+  Proof. clear.
+    induction b; simpl; intros; try congruence; auto.
+  Qed.
+
+  Fixpoint qsize (q : Quant) : nat :=
+    match q with
+      | QBase => 0
+      | QAll _ q              
+      | QEx _ q => S (qsize q)
+    end.
+
+  Lemma qsize_appendQ : forall a b,
+    qsize (appendQ a b) = qsize a + qsize b.
+  Proof.
+    clear; induction a; simpl in *; auto.
+  Qed.
+
+  Ltac apply_eq f H :=
+    match type of H with
+      | ?X = ?Y =>
+        assert (f X = f Y); [ f_equal; apply H | ] 
+    end.
+
+  Lemma appendQ_proper : forall a b c,
+    appendQ a b = appendQ c b ->
+    a = c.
+  Proof.
+    clear. induction a; destruct c; simpl; intros; try congruence;
+    repeat match goal with
+             | [ H : QAll _ _ = QAll _ _ |- _ ] => inversion H; clear H; subst
+             | [ H : QEx _ _ = QEx _ _ |- _ ] => inversion H; clear H; subst
+           end; try solve [ f_equal; eauto ]; exfalso.
+    { apply_eq qsize H. simpl in *; rewrite qsize_appendQ in H0. omega. }
+    { apply_eq qsize H. simpl in *; rewrite qsize_appendQ in H0. omega. }
+    { apply_eq qsize H. simpl in *; rewrite qsize_appendQ in H0. omega. }
+    { apply_eq qsize H. simpl in *; rewrite qsize_appendQ in H0. omega. }
+  Qed.
+
+End over_types.
